theories/caesium/loc.v
@@ -18,10 +18,10 @@ Definition dummy_alloc_id : alloc_id := 0.
 
 (** Provenances *)
 Inductive prov :=
-| ProvNull
-| ProvAlloc (aid : option alloc_id)
+| ProvNone
+| ProvAlloc (aid : alloc_id)
 | ProvFnPtr.
-Global Instance prov_inhabited : Inhabited prov := populate ProvNull.
+Global Instance prov_inhabited : Inhabited prov := populate ProvNone.
 Global Instance prov_eq_dec : EqDecision prov.
 Proof. solve_decision. Qed.
 Global Instance prov_countable : Countable prov.
@@ -29,28 +29,28 @@ Proof.
   refine (inj_countable'
     (λ prov,
      match prov with
-     | ProvNull => inl (inl tt)
+     | ProvNone => inl (inl tt)
      | ProvAlloc aid => inl (inr aid)
      | ProvFnPtr => inr tt
      end
     )
     (λ prov,
      match prov with
-     | inl (inl _) => ProvNull
+     | inl (inl _) => ProvNone
      | inl (inr aid) => ProvAlloc aid
      | inr _ => ProvFnPtr
      end) _); abstract by intros [].
 Defined.
 
 Definition prov_alloc_id (p : prov) : option alloc_id :=
-  if p is ProvAlloc aid then aid else None.
+  if p is ProvAlloc aid then Some aid else None.
 
 (** Memory location. *)
 Definition loc : Set := prov * addr.
 Bind Scope loc_scope with loc.
 
 Definition fn_loc (a : addr) : loc := (ProvFnPtr, a).
-Definition NULL_loc : loc := (ProvNull, 0).
+Definition NULL_loc : loc := (ProvNone, 0).
 Global Typeclasses Opaque NULL_loc fn_loc.
 
 (** Shifts location [l] by offset [z]. *)
