stdlib/ptr/output/ptr/proofs/proof_without_provenance_mut.v
@@ -1,7 +1,6 @@
 From caesium Require Import lang notation.
 From refinedrust Require Import typing shims.
 From rrstd.ptr.ptr.generated Require Import generated_code_ptr generated_specs_ptr generated_template_without_provenance_mut.
-From rrstd.ptr.ptr.proofs Require Import proof_invalid.
 
 Set Default Proof Using "Type".
 
@@ -11,6 +10,15 @@ Context `{RRGS : !refinedrustGS Σ}.
 Lemma without_provenance_mut_proof (π : thread_id) :
   without_provenance_mut_lemma π.
 Proof.
-  apply invalid_proof.
+  without_provenance_mut_prelude.
+
+  repeat liRStep. liShow.
+  set ((ProvNone, addr) : loc) as l.
+  repeat liRStep.
+
+  all: print_remaining_goal.
+  Unshelve. all: sidecond_solver.
+  Unshelve. all: sidecond_hammer.
+  Unshelve. all: print_remaining_sidecond.
 Qed.
 End proof.
